\GG{\partial_0 }{\partial_0 } & = \frac{3.0 \left(\frac{d}{d x_{0}} \phi{\left (x_{0} \right )}\right)^{2}}{\phi^{2}{\left (x_{0} \right )}} \\
\GG{\partial_0 }{\partial_1 } & = 0 \\
\GG{\partial_0 }{\partial_2 } & = 0 \\
\GG{\partial_0 }{\partial_3 } & = 0 \\
\GG{\partial_1 }{\partial_1 } & = \frac{\left(2.0 \phi{\left (x_{0} \right )} \frac{d^{2}}{d x_{0}^{2}} \phi{\left (x_{0} \right )} - 3.0 \left(\frac{d}{d x_{0}} \phi{\left (x_{0} \right )}\right)^{2}\right) \zeta_{1}{\left (x_{1} \right )}}{\phi^{2}{\left (x_{0} \right )}} \\
\GG{\partial_1 }{\partial_2 } & = 0 \\
\GG{\partial_1 }{\partial_3 } & = 0 \\
\GG{\partial_2 }{\partial_2 } & = \frac{\left(2.0 \phi{\left (x_{0} \right )} \frac{d^{2}}{d x_{0}^{2}} \phi{\left (x_{0} \right )} - 3.0 \left(\frac{d}{d x_{0}} \phi{\left (x_{0} \right )}\right)^{2}\right) \zeta_{2}{\left (x_{2} \right )}}{\phi^{2}{\left (x_{0} \right )}} \\
\GG{\partial_2 }{\partial_3 } & = 0 \\
\GG{\partial_3 }{\partial_3 } & = \frac{\left(2.0 \phi{\left (x_{0} \right )} \frac{d^{2}}{d x_{0}^{2}} \phi{\left (x_{0} \right )} - 3.0 \left(\frac{d}{d x_{0}} \phi{\left (x_{0} \right )}\right)^{2}\right) \zeta_{3}{\left (x_{3} \right )}}{\phi^{2}{\left (x_{0} \right )}} \\
